Finish preservation lemma

src/constr-dot/ConstrSafety.v
@@ -10,14 +10,152 @@ Require Import PreciseConstrTyping.
 Require Import ConstrWeakening ConstrNarrowing.
 Require Import ConstrBinding.
 Require Import InvertibleConstrTyping.
+Require Import ConstrSubstitution.
 Require Import ConstrCanonicalForms.
 
 (** The typing of a term with a stack *)
 Inductive constr_sta_trm_typ : sta * trm -> typ -> Prop :=
-| constr_sta_trm_typ_c : forall G s t T,
+| constr_sta_trm_typ_c : forall C G s t T,
     inert G ->
     G ⊨ C ->
-    well_typed G s ->
-    G ⊢ t : T ->
-    sta_trm_typ (s, t) T.
+    constr_well_typed C G s ->
+    (C, G) ⊢c t : T ->
+    constr_sta_trm_typ (s, t) T.
+
+Hint Constructors constr_sta_trm_typ.
+
+Notation "'⊢c' t ':' T" := (constr_sta_trm_typ t T) (at level 40, t at level 59).
+
+(** * Preservation *)
+
+(** If a value [v] has type [T], then [v] has a precise type [T']
+    that is a subtype of [T].
+    This lemma corresponds to Lemma 3.15 in the paper. *)
+Lemma constr_val_typing: forall C G v T,
+  (C, G) ⊢c trm_val v : T ->
+  exists T', (C, G) ⊢c!v v : T' /\
+        (C, G) ⊢c T' <: T.
+Proof.
+  introv H. dependent induction H; eauto using csubtyp_refl.
+  destruct (IHcty_trm _ _ _ eq_refl eq_refl). destruct_all.
+  eauto using constr_subtyping_trans.
+Qed.
+
+Ltac binds_eq :=
+  match goal with
+  | [Hb1: binds ?x _ ?G,
+     Hb2: binds ?x _ ?G |- _] =>
+     apply (binds_functional Hb1) in Hb2; inversions Hb2
+  end.
+
+Ltac invert_red :=
+  match goal with
+  | [Hr: (_, _) |-> (_, _) |- _] => inversions Hr
+  end.
+
+
+(** [s: G]                  #<br>#
+    [inert [G]              #<br>#
+    [(s, t) |-> (s', t')]   #<br>#
+    [G ⊢ t: T]              #<br>#
+    [―――――――――――――――――――]   #<br>#
+    [exists G', inert G']        #<br>#
+    [s': G, G']             #<br>#
+    [G, G' ⊢ t': T]         *)
+Lemma constr_preservation_helper: forall C G s t s' t' T,
+    constr_well_typed C G s ->
+    inert G ->
+    G ⊨ C ->
+    (s, t) |-> (s', t') ->
+    (C, G) ⊢c t : T ->
+    exists G', inert G' /\
+          (G & G') ⊨ C /\
+          constr_well_typed C (G & G') s' /\
+          (C, G & G') ⊢c t' : T.
+Proof.
+  introv Hwf Hin Hsat Hred Ht. gen t'.
+  dependent induction Ht; intros; try solve [invert_red].
+  - Case "ty_all_elim"%string.
+    match goal with
+    | [Hx: _ ⊢c trm_var (avar_f _) : typ_all _ _ |- _] =>
+        pose proof (constr_canonical_forms_fun Hin Hsat Hwf Hx) as [L [T' [t [Bis [Hsub Hty]]]]];
+        inversions Hred;
+        binds_eq
+    end.
+    exists (@empty typ). rewrite concat_empty_r. repeat_split_right; auto.
+    pick_fresh_gen (fv_ctx_types G \u fv_typ S \u fv_typ T \u fv_trm t0 \u fv_constr C \u L \u dom G) y.
+    assert (y \notin L) as FrL by auto. specialize (Hty y FrL).
+    apply* renaming_ctyp; eauto.
+  - Case "ty_new_elim"%string.
+    pose proof (constr_canonical_forms_obj Hin Hsat Hwf Ht) as [S [ds [t [Bis [Has Ty]]]]].
+    invert_red. binds_eq.
+    exists (@empty typ). rewrite concat_empty_r. repeat_split_right; auto.
+    rewrite* <- (defs_has_inv Has H5).
+  - Case "ty_let"%string.
+
+    Ltac solve_IH :=
+      match goal with
+      | [IH: forall G, inert _ ->
+            forall C, constr_well_typed _ _ _ ->
+            _ ⊨ _ ->
+            _ = _ ->
+            forall t', (_, _) |-> (_, _) -> _,
+          In: inert _,
+          Wf: constr_well_typed _ _ _,
+          Sat: _ ⊨ _,
+          Hr: (_, _) |-> (_, ?t') |- _] =>
+        idtac IH;
+        specialize (IH _ In _ Wf Sat eq_refl _ Hr); destruct_all
+      end;
+      match goal with
+      | [Hi: (_, _ & ?G') ⊢c _ : _ |- _] =>
+        exists G'; repeat_split_right; auto
+      end.
+
+    Ltac solve_let :=
+      invert_red; solve_IH; constr_fresh_constructor; eauto; try apply* weaken_constr_typing.
+
+    destruct t; try solve [solve_let].
+    + SCase "[t = (let x = a in u)] where a is a variable".
+      repeat invert_red.
+      exists (@empty typ). rewrite concat_empty_r. repeat_split_right; auto.
+      apply* constr_renaming_fresh.
+    + SCase "[t = (let x = v in u)] where v is a value".
+      repeat invert_red.
+      match goal with
+        | [Hn: ?x # ?s |- _] =>
+          pose proof (constr_well_typed_notin_dom Hwf Hn) as Hng
+      end.
+      pose proof (constr_val_typing Ht) as [V [Hv Hs]].
+      exists (x ~ V). repeat_split_right.
+      ** rewrite <- concat_empty_l. constructor~. apply (constr_precise_inert_typ Hv).
+      ** apply~ constr_satisfiable_push.
+      ** apply~ constr_well_typed_push. apply (constr_precise_to_general_v Hv).
+      ** eapply constr_renaming_fresh with (L:=L \u dom G \u \{x}). apply* ok_push.
+         intros. apply* weaken_constr_typing. apply cty_sub with (T:=V); auto. apply* weaken_csubtyp.
+  - Case "ty_sub"%string.
+    solve_IH.
+    match goal with
+    | [Hs: _ ⊢c _ <: _,
+       Hg: (_, _ & ?G') ⊢c _: _ |- _] =>
+      apply weaken_csubtyp with (G2:=G') in Hs;
+      eauto
+    end.
+Qed.
+
+(** ** Preservation Theorem *)
+
+(** [⊢ (s, t): T]           #<br>#
+    [(s, t) |-> (s', t')]   #<br>#
+    [―――――――――――――――――――]   #<br>#
+    [⊢ (s', t'): T]         *)
+Theorem constr_preservation : forall s s' t t' T,
+    ⊢c (s, t) : T ->
+    (s, t) |-> (s', t') ->
+    ⊢c (s', t') : T.
+Proof.
+  introv Ht Hr. destruct Ht as [* Hi Hsat Hwf Ht].
+  lets Hp: (constr_preservation_helper Hwf Hi Hsat Hr Ht). destruct Hp as [G' [Hi' [Hsat' [Hwf' Ht']]]].
+  apply constr_sta_trm_typ_c with (C:=C) (G:=G & G'); auto. apply* inert_concat.
+Qed.
 
